Veritas.Blum.fst
@@ -1,0 +1,111 @@
+module Veritas.Blum
+
+open FStar.Seq
+open Veritas.MultiSet
+open Veritas.MultiSetHash
+open Veritas.SeqAux
+open Veritas.Verifier
+open Veritas.Verifier.CorrectDefs
+
+(* get the add seq of a log *)
+let rec add_seq (il:t_verifiable_log): 
+  Tot (seq ms_hashfn_dom)
+  (decreases (tv_length il)) =
+  let (id,l) = il in
+  let n = length l in  
+  if n = 0 then 
+    Seq.empty #ms_hashfn_dom
+  else 
+    let l' = hprefix l in
+    let e = telem l in
+    match e with
+    | AddB r t j -> append1 (add_seq (id, l')) (MHDom r t j)
+    | _ ->  add_seq (id,l')
+
+(* get the add multi-set of a log *)
+let add_set (il:t_verifiable_log): mset ms_hashfn_dom = 
+  seq2mset (add_seq il)
+
+(* 
+ * the hadd hash value maintained by a verifier thread is the multiset hash 
+ * of its add_set 
+ *)
+let rec lemma_hadd_add_set (il:t_verifiable_log):
+  Lemma (requires True)
+        (ensures (thread_hadd (t_verify (fst il) (snd il)) = ms_hashfn (add_seq il))) 
+        (decreases (tv_length il)) =
+  let (id,l) = il in
+  let n = length l in
+  let st = t_verify id l in
+  if n = 0 then 
+    lemma_hashfn_empty()  
+  else (
+    let l' = hprefix l in
+    let e = telem l in
+    lemma_hadd_add_set (id, l');
+    match e with
+    | AddB r t j -> 
+           lemma_hashfn_app (add_seq (id, l')) (MHDom r t j)
+    | _ -> ()
+  )
+
+(* sequence of versioned records evicted from a verifier *)
+let rec evict_seq (il:t_verifiable_log):
+  Tot (seq ms_hashfn_dom)
+  (decreases (tv_length il)) = 
+  let (id,l) = il in
+  let n = length l in  
+  if n = 0 then 
+    Seq.empty #ms_hashfn_dom
+  else 
+    let (_,l') = tv_prefix il (n - 1) in
+    let e = telem l in
+    let vs' = t_verify id l' in
+    let st' = thread_store vs' in
+    match e with
+    | EvictB k t -> 
+      let v = stored_value st' k in 
+      append1 (evict_seq (id, l')) (MHDom (k,v) t id)
+    | EvictBM k k' t -> 
+      let v = stored_value st' k in 
+      append1 (evict_seq (id, l')) (MHDom (k,v) t id)    
+    | _ -> evict_seq (id, l')
+
+(* evict multiset of a verifier *)
+let evict_set (il:t_verifiable_log): mset ms_hashfn_dom =
+  seq2mset (evict_seq il)
+
+(* the thread id of a verifier remains unchanged *)
+let rec lemma_thread_id (il:t_verifiable_log):
+  Lemma (requires True)
+        (ensures (thread_id (t_verify (fst il) (snd il)) = (fst il)))
+        (decreases (tv_length il)) = 
+  let (id,l) = il in
+  let n = length l in
+  if n = 0 then ()
+  else
+    lemma_thread_id (id, hprefix l)
+
+let rec lemma_hevict_evict_set (il:t_verifiable_log):
+  Lemma (requires True)
+        (ensures (thread_hevict (t_verify (fst il) (snd il)) = ms_hashfn (evict_seq il)))
+        (decreases (tv_length il)) =
+  let (id, l) = il in
+  let n = length l in
+  if n = 0 then lemma_hashfn_empty()
+  else (
+    let l' = hprefix l in
+    let e = telem l in
+    let vs' = t_verify id l' in
+    let st' = thread_store vs' in    
+    lemma_hevict_evict_set (id, l');
+    lemma_thread_id (id, l');
+    match e with
+    | EvictB k t -> 
+      let v = stored_value st' k in
+      lemma_hashfn_app (evict_seq (id, l')) (MHDom (k,v) t id)
+    | EvictBM k _ t -> 
+      let v = stored_value st' k in
+      lemma_hashfn_app (evict_seq (id, l')) (MHDom (k,v) t id)
+    | _ -> ()
+  )
