Makefile
@@ -21,6 +21,7 @@ FSTAR_FILES := Veritas.BinTree.fsti Veritas.BinTree.fst \
                Veritas.Verifier.fst \
                Veritas.EAC.fst \
 	       Veritas.Verifier.CorrectDefs.fst \
+	       Veritas.Blum.fst \
                Veritas.Verifier.EAC.fst \
                Veritas.Verifier.Correctness.fst
 
